Word theories

opentheory/examples/all.ml
@@ -8,6 +8,9 @@ loads "opentheory/examples/parser.ml";;
 loads "opentheory/examples/modular.ml";;
 loads "opentheory/examples/word.ml";;
 loads "opentheory/examples/byte.ml";;
+loads "opentheory/examples/word16.ml";;
+(***
 loads "opentheory/examples/char.ml";;
+***)
 
 stop_logging ();;
