opentheory/examples/word.ml
@@ -2,6 +2,29 @@
 (* A functor theory of words.                                                *)
 (* ------------------------------------------------------------------------- *)
 
+logfile "list-interval-def";;
+
+let interval_def = new_recursive_definition num_RECURSION
+  `(interval m 0 = []) /\
+   (interval m (SUC n) = CONS m (interval (SUC m) n))`;;
+
+export_thm interval_def;;
+
+logfile "list-zipwith-def";;
+
+let zipwith_raw_def = new_recursive_definition list_RECURSION
+  `(zipwith f [] l = []) /\
+   (zipwith f (CONS h t) l = CONS (f h (HD l)) (zipwith f t (TL l)))`;;
+
+let zipwith_def = prove
+   (`(!f. zipwith (f : A -> B -> C) [] [] = []) /\
+     (!f h1 h2 t1 t2.
+        zipwith (f : A -> B -> C) (CONS h1 t1) (CONS h2 t2) =
+        CONS (f h1 h2) (zipwith f t1 t2))`,
+    REWRITE_TAC [zipwith_raw_def; HD; TL]);;
+
+export_thm zipwith_def;;
+
 new_constant ("word_width", `:num`);;
 
 logfile "word-def";;
@@ -22,19 +45,60 @@ export_thm word_size_nonzero;;
 
 new_type ("word",0);;
 
+new_constant ("word_add", `:word -> word -> word`);;
+new_constant ("word_mult", `:word -> word -> word`);;
+new_constant ("word_neg", `:word -> word`);;
+new_constant ("word_sub", `:word -> word -> word`);;
+new_constant ("word_le", `:word -> word -> bool`);;
+new_constant ("word_lt", `:word -> word -> bool`);;
+new_constant ("num_to_word", `:num -> word`);;
 new_constant ("word_to_num", `:word -> num`);;
 
 logfile "word-bits";;
 
-let word_to_list_f_def = new_recursive_definition num_RECURSION
- `(!k. word_to_list_f 0 k = []) /\
-  (!n k. word_to_list_f (SUC n) k = CONS (ODD k) (word_to_list_f n (k DIV 2)))`;;
+let word_shl_def = new_definition
+ `word_shl w n = num_to_word (word_to_num w * (2 EXP n))`;;
 
-export_thm word_to_list_f_def;;
+export_thm word_shl_def;;
+
+let word_shr_def = new_definition
+ `word_shr w n = num_to_word (word_to_num w DIV (2 EXP n))`;;
+
+export_thm word_shr_def;;
+
+let word_bit_def = new_definition
+ `word_bit w n = ODD (word_to_num (word_shr w n))`;;
+
+export_thm word_bit_def;;
 
 let word_to_list_def = new_definition
-  `word_to_list w = word_to_list_f word_width (word_to_num w)`;;
+ `word_to_list w = MAP (word_bit w) (interval 0 word_width)`;;
 
 export_thm word_to_list_def;;
+
+let list_to_word_def = new_recursive_definition list_RECURSION
+  `(list_to_word [] = num_to_word 0) /\
+   (list_to_word (CONS h t) =
+    if h then word_add (word_shl (list_to_word t) 1) (num_to_word 1)
+    else word_shl (list_to_word t) 1)`;;
+
+export_thm list_to_word_def;;
+
+let word_and_def = new_definition
+  `word_and w1 w2 =
+   list_to_word (zipwith ( /\ ) (word_to_list w1) (word_to_list w2))`;;
+
+export_thm word_and_def;;
+
+let word_or_def = new_definition
+  `word_or w1 w2 =
+   list_to_word (zipwith ( \/ ) (word_to_list w1) (word_to_list w2))`;;
+
+export_thm word_or_def;;
+
+let word_not_def = new_definition
+  `word_not w = list_to_word (MAP (~) (word_to_list w))`;;
+
+export_thm word_not_def;;
 
 logfile_end ();;
