opentheory/examples/byte.ml
@@ -10,3 +10,25 @@ let byte_width_def = new_definition
 export_thm byte_width_def;;
 
 logfile_end ();;
+
+(* Apply theory functor word *)
+
+new_type ("byte",0);;
+
+new_constant ("byte_add", `:byte -> byte -> byte`);;
+new_constant ("byte_mult", `:byte -> byte -> byte`);;
+new_constant ("byte_neg", `:byte -> byte`);;
+new_constant ("byte_sub", `:byte -> byte -> byte`);;
+new_constant ("byte_le", `:byte -> byte -> bool`);;
+new_constant ("byte_lt", `:byte -> byte -> bool`);;
+new_constant ("byte_and", `:byte -> byte -> byte`);;
+new_constant ("byte_bit", `:byte -> num -> bool`);;
+new_constant ("list_to_byte", `:bool list -> byte`);;
+new_constant ("num_to_byte", `:num -> byte`);;
+new_constant ("byte_not", `:byte -> byte`);;
+new_constant ("byte_or", `:byte -> byte -> byte`);;
+new_constant ("byte_shl", `:byte -> num -> byte`);;
+new_constant ("byte_shr", `:byte -> num -> byte`);;
+new_constant ("byte_size", `:num`);;
+new_constant ("byte_to_list", `:byte -> bool list`);;
+new_constant ("byte_to_num", `:byte -> num`);;
