opentheory/examples/word16.ml
@@ -1,0 +1,54 @@
+(* ------------------------------------------------------------------------- *)
+(* A type of 16-bit words.                                                   *)
+(* ------------------------------------------------------------------------- *)
+
+logfile "word16-def";;
+
+let word16_width_def = new_definition
+  `word16_width = 16`;;
+
+export_thm word16_width_def;;
+
+logfile_end ();;
+
+(* Apply theory functor word *)
+
+new_type ("word16",0);;
+
+new_constant ("word16_add", `:word16 -> word16 -> word16`);;
+new_constant ("word16_mult", `:word16 -> word16 -> word16`);;
+new_constant ("word16_neg", `:word16 -> word16`);;
+new_constant ("word16_sub", `:word16 -> word16 -> word16`);;
+new_constant ("word16_le", `:word16 -> word16 -> bool`);;
+new_constant ("word16_lt", `:word16 -> word16 -> bool`);;
+new_constant ("word16_and", `:word16 -> word16 -> word16`);;
+new_constant ("word16_bit", `:word16 -> num -> bool`);;
+new_constant ("list_to_word16", `:bool list -> word16`);;
+new_constant ("num_to_word16", `:num -> word16`);;
+new_constant ("word16_not", `:word16 -> word16`);;
+new_constant ("word16_or", `:word16 -> word16 -> word16`);;
+new_constant ("word16_shl", `:word16 -> num -> word16`);;
+new_constant ("word16_shr", `:word16 -> num -> word16`);;
+new_constant ("word16_size", `:num`);;
+new_constant ("word16_to_list", `:word16 -> bool list`);;
+new_constant ("word16_to_num", `:word16 -> num`);;
+
+logfile "word16-bytes";;
+
+let word16_to_bytes_def = new_definition
+  `word16_to_bytes w =
+     (num_to_byte (word16_to_num (word16_shr w 8)),
+      num_to_byte (word16_to_num (word16_and w (num_to_word16 255))))`;;
+
+export_thm word16_to_bytes_def;;
+
+let bytes_to_word16_def = new_definition
+  `bytes_to_word16 b1 b2 =
+     word16_or
+       (word16_shl (num_to_word16 (byte_to_num b1)) 8)
+       (num_to_word16 (byte_to_num b2))`;;
+
+export_thm bytes_to_word16_def;;
+
+logfile_end ();;
+
